%%%%%%%%%%%%%%%%%%%%%%%
\item
%%%%%%%%%%%%%%%%%%%%%%%

Following the argument of  \refprob~7--10, we know that the Wronskian satisfies
\[
    W'(x) = \frac{2x}{1 - x^2} W(x).
\]
\[
    \Rightarrow W(x)
    = P_l(x) Q_l'(x) - P_l'(x) Q_l(x)
    = \frac{C_l}{1 - x^2}
\]
\[
    \Rightarrow C_l
    = \left( 1 - x^2 \right) \left(
        P_l(x) Q_l'(x) - P_l'(x) Q_l(x)
    \right).
\]
This time, let us find $C_l$ using the asymptotic behavior at infinity.
\begin{align*}
    P_l(x)
    &= \inv{2^l l!} \frac{d^l}{dx^l} {\left( x^2 - 1 \right)}^l \\
    &\sim \inv{2^l l!} \frac{d^l}{dx^l} x^{2l} \\
    &= \frac{(2l)!}{2^l {(l!)}^2} x^{l}
\end{align*}
\begin{align*}
    Q_l(x)
    &= - P_l(x) \int^x \frac{dx}{\left( x^2 - 1 \right) {P_l(x)}^2} \\
    &\sim -\frac{(2l)!}{2^l {(l!)}^2} x^{l} \cdot \int^x \frac{dx}{
        x^2 {\left( \frac{(2l)!}{2^l {(l!)}^2} x^{l} \right)}^2
    } \\
    &= -\frac{2^l {(l!)}^2}{(2l)!} x^l \int^x \frac{dx}{x^{2l+2}} \\
    &= \frac{2^l {(l!)}^2}{(2l + 1) (2l)!} x^{-l-1}
\end{align*}
\begin{align*}
    \Rightarrow C_l
    &= \lim_{x \rightarrow \infty} \left( 1 - x^2 \right) \left(
        P_l(x) Q_l'(x) - P_l'(x) Q_l(x)
    \right) \\
    &= -\lim_{x \rightarrow \infty} x^2 \left(
        -\frac{(2l)!}{2^l {(l!)}^2} x^{l} \cdot \frac{(l + 1) 2^l {(l!)}^2}{(2l + 1) (2l)!} x^{-l-2} 
    \right. \\
    &\quad \left.
        - \frac{(2l)!}{2^l {(l!)}^2} lx^{l - 1} \cdot \frac{2^l {(l!)}^2}{(2l + 1) (2l)!} x^{-l-1}
    \right) \\
    &= 1
\end{align*}
\[
    \therefore W(x) = \inv{1 - x^2}
\]
