%%%%%%%%%%%%%%%%%%%%%%%
\item
%%%%%%%%%%%%%%%%%%%%%%%

The differential equation is given by
\begin{align*}
    0
    &= {\left( \beta x^\gamma \right)}^2 \frac{d^2}{d{\left( \beta x^\gamma \right)}^2} \left( x^{-\alpha} y \right)
     - 2\left( \beta x^\gamma \right) \frac{d}{d\left( \beta x^\gamma \right)} \left( x^{-\alpha} y \right) \\
    &\quad + \left( {\left( \beta x^\gamma \right)}^2 - m^2 \right) \left( x^{-\alpha} y \right).
\end{align*}
\begin{align*}
    \frac{d}{d\left( \beta x^\gamma \right)} \left( x^{-\alpha} y \right)
    &= \inv{\beta\gamma x^{\gamma - 1}} \frac{d}{dx} \left( x^{-\alpha} y \right) \\
    &= \inv{\beta\gamma x^{\gamma - 1}} \left(
        x^{-\alpha} y' - \alpha x^{-\alpha - 1} y
    \right) \\
    &= \inv{\beta\gamma} \left(
        x^{-\alpha-\gamma+1} y' - \alpha x^{-\alpha-\gamma} y
    \right)
\end{align*}
\begin{align*}
    \Rightarrow
    &\frac{d^2}{d{\left( \beta x^\gamma \right)}^2} \left( x^{-\alpha} y \right) \\
    &= \inv{\beta\gamma x^{\gamma - 1}} \frac{d}{dx} \left(
        \inv{\beta\gamma} \left(
            x^{-\alpha-\gamma+1} y' - \alpha x^{-\alpha-\gamma} y
        \right)
    \right) \\
    &= \inv{\beta^2 \gamma^2} \left(
        x^{-\alpha-2\gamma+2} y''
        - (2\alpha+\gamma-1) x^{-\alpha-2\gamma+1} y'
        + \alpha(\alpha + \gamma) x^{-\alpha-2\gamma} y
    \right)
\end{align*}
\begin{align*}
    \Rightarrow 0
    &= \inv{\gamma^2 x^{\alpha}} \left(
        x^2 y'' - (2\alpha+\gamma-1) xy' + \alpha(\alpha+\gamma) y
    \right) \\
    &\quad - \frac{2}{\gamma x^{\alpha}} \left(
        xy' - \alpha y
    \right) \\
    &\quad + \frac{{\left( \beta x^\gamma \right)}^2 - m^2}{x^\alpha} y \\
    &= \inv{\gamma^2 x^{-\alpha}} \left(
        x^2 y''
        - (2\alpha - 1) y'
        + \left( \beta^2 \gamma^2 x^{2\gamma} + \alpha^2 - m^2 \gamma^2 \right)
    \right)
\end{align*}
\[
    \therefore  x^2 y''
    - (2\alpha - 1) y'
    + \left( \beta^2 \gamma^2 x^{2\gamma} + \alpha^2 - m^2 \gamma^2 \right)
    = 0
\]
As a sanity check, substituting $\alpha = 0,\; \beta =\gamma = 1$ yields
the original Bessel equation.

The equation
\[
    y'' + x^2 y = 0
\]
can be obtained via the substitution $\alpha =\beta = \half,\; \gamma = 2, m = \inv{4}$.
\[
    \therefore y
    = C_1 \sqrt{x} J_{\inv{4}}\left( \half x^2 \right)
    + C_2 \sqrt{x} J_{-\inv{4}}\left( \half x^2 \right)
\]
