%%%%%%%%%%%%%%%%%%%%%%%
\item
%%%%%%%%%%%%%%%%%%%%%%%

Without loss of generality, we may only prove the statement for $m \geq 0$.
\begin{align*}
    J_{-m}(x)
    &= \sum_{r = 0}^\infty \frac{{(-1)}^r}{r! \Gamma(r -m + 1)}
       {\left( \frac{x}{2} \right)}^{-m + 2r} \\
    &= \sum_{r = m}^\infty \frac{{(-1)}^r}{r! (r - m)!}
       {\left( \frac{x}{2} \right)}^{-m + 2r} \\
    &= \sum_{r = 0}^\infty \frac{{(-1)}^{r + m}}{(r + m)! r!}
       {\left( \frac{x}{2} \right)}^{-m + 2r + 2m} \\
    &= {(-1)}^m \sum_{r = 0}^\infty
       \frac{{(-1)}^r}{r! \Gamma(r + m + 1)}
       {\left( \frac{x}{2} \right)}^{m + 2r} \\
    &= {(-1)}^m J_m(x)
\end{align*}
