%%%%%%%%%%%%%%%%%%%%%%%
\item
%%%%%%%%%%%%%%%%%%%%%%%

We transpose the two regular singularities 0 and 1 with the transformation $u = 1 - z$.
This transforms the hypergeometric equation as
\[
    u (1 - u) \frac{d^2 y}{du^2}
    + \left( -c - (a + b + 1) u \right) \frac{dy}{du}
    - ab y
    = 0.
\]
\begin{align*}
    \Rightarrow y
    &= C_1 \hypergeom (a, b; -c; u) \\
    &\quad + C_2 u^{1 + c} \hypergeom (1+a+c, 1+b+c; 2+c; u) \\
    &= C_1 \hypergeom(a, b; -c; 1-z) \\
    &\quad + C_2 {(1 - z)}^{1 + c} \hypergeom (1+a+c, 1+b+c; 2+c; 1-z)
\end{align*}
