%%%%%%%%%%%%%%%%%%%%%%%
\item
%%%%%%%%%%%%%%%%%%%%%%%

\begin{enumerate}[wide, labelindent = 0pt, label = (\alph*)]
\item
\begin{align*}
    \sum_{n = 0}^\infty H_{n + 1}(x) \frac{h^n}{n!}
    &= \partialderiv{h} \left(
        \sum_{n = 0}^\infty H_n(x) \frac{h^n}{n!}
    \right) \\
    &= \partialderiv{h} e^{2hx - h^2} \\
    &= 2 (x - h) e^{2hx - h^2} \\
    &= 2 (x - h) \sum_{n = 0}^\infty H_n(x) \frac{h^n}{n!} \\
    &= \sum_{n = 0}^\infty 2\left(
        xH_n(x) - nH_{n - 1}(x)
    \right) \frac{h^n}{n!}
\end{align*}
\[
    \therefore H_{n + 1} = 2xH_n(x) - 2nH_{n - 1}(x)
\]

\item
\begin{align*}
    \sum_{n = 0}^\infty \frac{h^n}{n!}
    \int_{-\infty}^\infty dx e^{-\frac{x^2}{2}} H_n(x)
    &= \int_{-\infty}^\infty dx e^{-\frac{x^2}{2}} \left(
        \sum_{n = 0}^\infty H_n(x) \frac{h^n}{n!}
    \right) \\
    &= \int_{-\infty}^\infty dx e^{-\frac{x^2}{2} + 2hx - h^2} \\
    &= \int_{-\infty}^\infty dx e^{-\frac{x^2}{2}} e^{
        -\half {(x - 2h)}^2 + h^2
    } \\
    &= \sqrt{2\pi} e^{h^2} \\
    &= \sum_{n = 0}^\infty \frac{\sqrt{2\pi}}{n!} h^{2n}
\end{align*}
\[
    \therefore \int_{-\infty}^\infty dx e^{-\frac{x^2}{2}} H_n(x) =
    \begin{cases}
        0 & (2 \nmid n) \\
        \frac{\sqrt{2\pi} n!}{\left( \frac{n}{2} \right)!} & (2 \mid n)
    \end{cases}
\]
\end{enumerate}