%%%%%%%%%%%%%%%%%%%%%%%
\item
%%%%%%%%%%%%%%%%%%%%%%%

\begin{enumerate}[wide, labelindent = 0pt, label = (\alph*)]
\item
\begin{align*}
    J_{\half}(x)
    &= \sum_{r = 0}^\infty \frac{{(-1)}^r}{r!\Gamma\left( r + \frac{3}{2} \right)} {\left( \frac{x}{2} \right)}^{\half + 2r} \\
    &= \inv{\sqrt{\pi}} \sum_{r = 0}^\infty \frac{{(-1)}^r}{
        r! \prod_{j = 0}^r \left( \half + j \right)
    } {\left( \frac{x}{2} \right)}^{\half + 2r} \\
    &= \inv{\frac{2}{\pi}} \sum_{r = 0}^\infty \frac{{(-1)}^r}{
        2^r r! (2r + 1)!!
    } x^{\half + 2r} \\
    &= \sqrt{\frac{2}{\pi x}} \sum_{r = 0}^\infty
       \frac{{(-1)}^r}{(2r + 1)!} x^{2r + 1} \\
    &= \sqrt{\frac{2}{\pi x}} \sin x
\end{align*}

\item
\begin{align*}
    J_{-\half}
    &= \frac{\half}{x} J_{\half}(x) + J_{\half}'(x) \\
    &= \inv{\sqrt{2\pi x^3}} \sin x + \sqrt{\frac{2}{\pi}} \left(
        -\half x^{-\frac{3}{2}} \sin x + x^{-\half} \cos x
    \right) \\
    &= \sqrt{\frac{2}{\pi x}} \cos x
\end{align*}

\end{enumerate}
