%%%%%%%%%%%%%%%%%%%%%%%
\item
%%%%%%%%%%%%%%%%%%%%%%%

Recall that
\[
    Y_{lm}(\Omega)
    = {\left( \frac{2l + 1}{4\pi} \frac{(l - \abs{m})!}{(l + \abs{m})!} \right)}^{\half}
       P_l^{\abs{m}}(\cos\theta) e^{im\phi}
       \times \begin{cases}
           {(-1)}^m & (m \geq 0) \\
           1        & (m < 0)
       \end{cases}.
\]
\begin{enumerate}[wide, labelindent = 0pt, label = (\roman*)]
\item $m \geq 0$:
\begin{align*}
    {(-1)}^m P_l^m(\cos\theta)
    &= \frac{{(-1)}^m}{2^l l!} {\left( 1- \cos^2\theta \right)}^{\frac{m}{2}}
       \frac{d^{l + m}}{d{(\cos\theta)^{l + m}}}
       {\left( \cos^2\theta - 1 \right)}^l \\
    &= \inv{2^l l!} {\left( -\sin\theta \right)}^m
       \frac{d^{l + m}}{d{(\cos\theta)^{l + m}}}
       {\left( \cos^2\theta - 1 \right)}^l
\end{align*}

\item $m < 0$:
\notyet
\end{enumerate}