%%%%%%%%%%%%%%%%%%%%%%%
\item
%%%%%%%%%%%%%%%%%%%%%%%

We use the recursion formulae derived from \refeq{7}{129}:
\[
    B_3 = \left( \frac{2}{\beta} \left( \alpha - 1 \right) + 1 \right) B_1,\;
    B_{n + 2} = \frac{2}{\beta} \left( n^2 - \alpha \right) B_n - B_{n - 2}
\]
as the $se_{2n + 1}(x)$ solutions contain $B_{2n + 1}$ terms.
\begin{align*}
    \frac{B_n}{B_{n - 2}}
    &= \cfrac{1}{
        \cfrac{2}{\beta} \left( n^2 - \alpha^2 \right)
        - \cfrac{B_{n + 2}}{B_n}
    } \\
    &= \cfrac{-\beta}{
        2\left( \alpha^2 - n^2 \right)
        + \beta \cfrac{B_{n + 2}}{B_n}
    } \\
    &= \cfrac{-\beta}{
        2\left( \alpha^2 - n^2 \right)
        - \cfrac{\beta^2}{
            2\left( \alpha^2 - {(n + 1)}^2 \right)
            - \cfrac{\beta^2}{\ddots}
        }
    }
\end{align*}
\begin{align*}
    \Rightarrow \frac{B_3}{B_1}
    &= \frac{2}{\beta} \left( 1 - \alpha \right) + 1 \\
    &= \cfrac{-\beta}{
        2\left( \alpha^2 - 9 \right)
        - \cfrac{\beta^2}{
            2\left( \alpha^2 - 16 \right)
            - \cfrac{\beta^2}{\ddots}
        }
    }
\end{align*}
\[
    \therefore \alpha(\beta)
    = 1 + \frac{\beta}{2} + \cfrac{\beta^2 / 2}{
        2\left( \alpha^2 - 9 \right)
        - \cfrac{\beta^2}{
            2 \left( \alpha^2 - 25 \right)
            - \cfrac{\beta^2}{\ddots}
        }
    }
\]

$se_1(x)$ has $\alpha = 1$ for $\beta = 0$.
\[
    \Rightarrow \alpha
    \approx 1 + \frac{\beta}{2}
\]
\[
    \Rightarrow \alpha
    \approx 1 + \frac{\beta}{2} + \frac{\beta^2 / 2}{2(1 - 9)}
    = 1 + \frac{\beta}{2} - \frac{\beta^2}{16}
\]
\[
    \Rightarrow \alpha
    \approx 1 + \frac{\beta}{2} + \cfrac{\beta^2 / 2}{
        2\left( {\left( 1 + \cfrac{\beta}{2} \right)}^2 - 9 \right)
        - \cfrac{\beta^2}{2(1 - 25)}
    }
    \approx 1 + \frac{\beta}{2} - \frac{\beta^2}{32} - \frac{\beta^3    }{256}
\]
