%%%%%%%%%%%%%%%%%%%%%%%
\item
%%%%%%%%%%%%%%%%%%%%%%%

Let us denote the Legendre coefficients as $\{c_n\}$.
\begin{align*}
    c_n
    &= \frac{2n + 1}{2} \int_{-1}^1 dx P_n (x) f(x) \\
    &= \frac{2n + 1}{2} \left(
        - \int_{-1}^0 dx P_n (x)
        + \int_0   ^1 dx P_n (x)
    \right) \\
    &= \frac{2n + 1}{2} \left(
        -{(-1)}^n + 1
    \right) \int_0^1 dx P_n(x) \\
    &= \begin{cases}
        0                           & (2 \mid  n) \\
        (2n + 1) \int_0^1 dx P_n(x) & (2 \nmid n)
    \end{cases}
\end{align*}
To evaluate the integral, we use the generating function.
\begin{align*}
    \sum_{n = 0}^\infty h^n \int_0^1 dx P_n(x)
    &= \int_0^1 dx \left(
        \sum_{n=0}^\infty h^n P_n(x)
    \right) \\
    &= \int_0^1 \frac{dx}{
        \sqrt{1 - 2hx + h^2}
    } \\
    &= \diffBetween{-\frac{\sqrt{1 - 2hx + h^2}}{h}}{0}{1} \\
    &= \frac{\sqrt{1 + h^2} - (1 - h)}{h} \\
    &= \inv{h} \left(
        \sum_{l=0}^\infty \binom{\half}{l}h^{2l} - 1 + h
    \right) \\
    &= 1 + \sum_{l = 1}^\infty \binom{\half}{l} h^{2l - 1}
\end{align*}
Here, we used the fact that $\abs{h} < 1$.
\begin{align*}
    \Rightarrow c_{2l + 1}
    &= (4l + 3) \binom{\half}{l + 1} \\
    &= (4l + 3) \frac{
        \prod_{j=0}^l \left( \half - j \right)
    }{(l + 1)!} \\
    &= (4l + 3) \frac{
        {(-1)}^{l + 1} \prod_{j=0}^l (2j - 1)
    }{2^{l + 1} (l+1)!} \\
    &= {(-1)}^l (4l + 3) \frac{(2l - 1)!!}{(2l + 2)!!}
\end{align*}
\begin{align*}
    \therefore f(x)
    &= \sum_{n=0}^\infty {(-1)}^n (4n + 3) \frac{(2n - 1)!!}{(2n + 2)!!} P_n(x) \\
    &= \frac{3}{2}    P_1(x)
     - \frac{7}{8}    P_3(x)
     + \frac{11}{16}  P_5(x)
     - \frac{75}{128} P_7(x)
     + \cdots
\end{align*}
