%%%%%%%%%%%%%%%%%%%%%%%
\item
%%%%%%%%%%%%%%%%%%%%%%%

\begin{enumerate}[wide, labelindent = 0pt, label = (\arabic*)]
\item 
We will make the change of variables
\[
    x = \cos\alpha \text{ and } y=\cos\beta.
\]
Without loss of generality, suppose we have defined the coordinate system
such that the direction for $\alpha$ is parallel to the $z$ axis
and that for $\beta$ lies in the $zx$ plane.
The coordinates $(x, y)$ maps to exactly two points on the unit sphere,
where the two points have the same $\theta$ but $\phi$'s that add to $2\pi$.
(In a coordinate-independent formulation, $(x, y)$ represents a unique point
on one of the two half-spheres cut by the plane containing the two fixed directions.)
The integrals evaluated on each half-sphere are equal,
so we may perform the change of variables for one of the half-spheres
and multiply the result by 2.

Let $\gamma$ denote the angle between the two fixed directions.
\[
    x = \cos\theta,\;
    y = \cos\gamma\cos\theta + \sin\gamma\sin\theta\cos\phi.
\]
\[
    \Rightarrow \begin{cases}
        \cos\theta = x & \sin\theta = \sqrt{1 - x^2} \\
        \cos\phi = \frac{y - x\cos\gamma}{\sin\gamma \sqrt{1 - x^2}}
    \end{cases}
\]
\begin{align*}
    \Rightarrow \frac{\partial(x, y)}{\partial(\theta,\phi)}
    &= \begin{vmatrix}
        \frac{\partial x}{\partial \theta} & \frac{\partial x}{\partial \phi} \\
        \frac{\partial y}{\partial \theta} & \frac{\partial y}{\partial \phi}
    \end{vmatrix} \\
    &= \sin\gamma \sin^2 \theta \sin\phi \\
    &= \sin\gamma \left( 1 - x^2 \right) \sqrt{
        1 - {\left(
            \frac{y - x\cos\gamma}{\sin\gamma \sqrt{1 - x^2}} 
        \right)}^2
    } \\
    &= \sqrt{\left( 1 - x^2 \right) \left(
        \sin^2 \gamma - x^2 - y^2 + 2xy\cos\gamma
    \right)}
\end{align*}
\[
    \therefore I
    = \int_{-1}^1 dx \int_{-1}^1 dy f(x) g(y) \cdot \frac{2}{
        \sqrt{\left( 1 - x^2 \right) \left(
            \sin^2 \gamma - x^2 - y^2 + 2xy\cos\gamma
        \right)}
    }
\]

\item
\notyet
\end{enumerate}