%%%%%%%%%%%%%%%%%%%%%%%
\item
%%%%%%%%%%%%%%%%%%%%%%%

Following the discussion in \refprob~7--10, the Wronskian must satisfy
\[
    W'(z)
    = -\frac{c - z}{z} W(z)
    = \left( -\frac{c}{z} + 1 \right) W(z).
\]
\[
    \Rightarrow W(z)
    = C z^{-c} e^{-z}
\]
\begin{align*}
    \Rightarrow C
    &= \lim_{z \rightarrow 0} z^c \left(
        \confhypergeom (a; c; z) \left(
            z^{1 - c} \confhypergeom (1 + a - c; 2 - c; z)
        \right)'
    \right. \\
    &\quad \left.
        - \confhypergeom' (a; c; z) \cdot z^{1 - c} \confhypergeom (1 + a - c; 2 - c; z)
    \right) \\
    &= 1 - c
\end{align*}
\[
    \therefore W(z) = (1 - c) z^{-c} e^z
\]