%%%%%%%%%%%%%%%%%%%%%%%
23.
%%%%%%%%%%%%%%%%%%%%%%%
The clever idea here is that we could make a variable change from $x$ to $u$,
where we could choose $u$ so as to make the equation easier to solve.
\begin{align*}
	0
	 & = A \frac{d^2 y}{dx^2} + \frac{dA}{dx} \frac{dy}{dx} + \frac{y}{A}        \\
	 & = A \frac{du}{dx} \frac{d}{du} \left( \frac{du}{dx} \frac{dy}{dy} \right)
	+ \frac{dA}{dx} \frac{du}{dx} \frac{dy}{du} + \frac{y}{A}                    \\
	 & = A {\left( \frac{du}{dx} \right)}^2 \frac{d^2 y}{du^2}
	+ \frac{dy}{du} \frac{d}{dx} \left( A \frac{dy}{dx} \right)
\end{align*}
Thus, we could define $\frac{du}{dx} = \frac{1}{A(x)}$ or $u = \int \frac{dx}{A(x)}$ to obtain
\[
	\frac{d^2 y}{du^2} = -y
	\Rightarrow y(u) = C_1 \cos \left( u + C_2 \right)
\]
\[
	\therefore y(x) = C_1 \cos \left( \int \frac{dx}{A(x)} + C_2 \right)
\]
