%%%%%%%%%%%%%%%%%%%%%%%
38.
%%%%%%%%%%%%%%%%%%%%%%
\begin{enumerate}[wide, labelindent=0pt, label= (\alph*)]
	\item
	      Let $y := \sum_{n=1}^\infty c_n {(x - 1)}^n$.
	      \begin{align*}
		      e^{y/x}
		       & = \sum_{n=0}^\infty \frac{1}{n!} {\left( \frac{y}{x} \right)}^n
		      = \sum_{n=0}^\infty\frac{y^n}{n!} {\left( 1 + \left( x - 1 \right) \right)}^{-n}                \\
		       & = \sum_{n=0}^\infty\frac{y^n}{n!} \left( \sum_{m=0}^\infty \binom{-n}{m} {(x - 1)}^m \right) \\
		       & = 1 + \sum_{m=0}^2 \binom{-1}{m} {(x - 1)}^m y
		      + \sum_{m=0}^1 \binom{-2}{m} {(x - 1)}^m \frac{y^2}{2}
		      + \frac{y^3}{6}
		      + O \left( {(x - 1)}^4 \right)                                                                  \\
		       & = 1 + c_1 (x - 1)
		      + \left( c_2 - c_1 + \frac{c_1^2}{2} \right) {(x - 1)}^2                                        \\
		       & \;\;\;\;+ \left( c_3 - c_2 + c_1 - c_1 c_2 - c_1^2 + \frac{c_1^3}{6} \right) {(x - 1)}^3
		      + O \left( {(x - 1)}^4 \right)
	      \end{align*}
	      Comparing this with
	      \[
		      y' = c_1 + 2c_2 (x - 1) + 3c_3 {(x - 1)}^2 + O \left( {(x - 1)}^3 \right),
	      \]
	      we can see that
	      \[
		      c_1 = 1,\;
		      c_2 = \frac{c_1}{2} = \half,\;
		      c_3 = \frac{1}{3} \left( c_2 - c_1 + \frac{c_1^2}{2} \right) = 0
	      \]
	      \[
		      \therefore y = (x - 1) + \half {(x - 1)}^2 + O \left( {(x - 1)}^4 \right)
	      \]

	\item
	      Let $y = xv$.
	      \[
		      xv' + v = e^v
		      \Rightarrow \frac{dv}{e^v - v} = \frac{dx}{x}
		      \Rightarrow \int_1^{y/x} \frac{dv}{e^v - v} = \ln x + C_1
	      \]
	      \[
		      \ln x_0 + C_1 = \int_1^\infty \frac{dv}{e^v - v} =: \alpha
		      \Rightarrow C_1 = \alpha - \ln x_0
	      \]
	      \[
		      \int_1^{y/x} \frac{dv}{e^v - v} = \ln \frac{x}{x_0} + \alpha
		      \Rightarrow \int_{y/x}^\infty \frac{dv}{e^v - v} = -\ln \frac{x}{x_0}
	      \]
	      For values of $x$ slightly less than $x_0$, we have $\frac{y}{x} >> 1$.
	      \[
		      \Rightarrow -\ln \frac{x}{x_0} \approx \int_{y/x}^\infty dv e^{-v} = e^{-y/x}
	      \]
	      \[
		      \therefore y \approx -x \ln \ln \frac{x_0}{x}
	      \]

\end{enumerate}
