%%%%%%%%%%%%%%%%%%%%%%%
12.
%%%%%%%%%%%%%%%%%%%%%%%
We define the integrating factor $\lambda$:
\[
	\lambda = \exp \left( \int \frac{dx}{1 + x^2} \right) = \exp \left( \tan^{-1} x \right)
\]
\[
	\Rightarrow \left( \exp \left( \tan^{-1} x \right) y \right)'
	= \frac{1}{1 + x^2} \cdot \tan^{-1} x \cdot \exp \left( \tan^{-1} x \right)
\]
\[
	\Rightarrow \exp \left( \tan^{-1} x \right) y
	= \left( \tan^{-1}x - 1 \right) \exp \left( \tan^{-1} x \right) + C
\]
\[
	\therefore y = C \exp \left( -\tan^{-1} x \right) + \tan^{-1} x - 1
\]
