%%%%%%%%%%%%%%%%%%%%%%%
3.
%%%%%%%%%%%%%%%%%%%%%%%
\begin{enumerate}[wide, labelindent = 0pt, label = (\alph*)]
\item
\begin{align*}
    {\left( C^{-1} A C \right)}^\dagger
    &= C^\dagger A^\dagger {\left( C^{-1} \right)}^\dagger \\
    &= C^{-1} A {\left( C^{-1} \right)}^\dagger
\end{align*}
Now, notice that for a general invertible matrix $M$,
\begin{align*}
    {\left( M^{-1} \right)}^\dagger M^\dagger
    &= {\left( M M^{-1} \right)}^\dagger \\
    &= 1^\dagger \\
    &= 1
\end{align*}
and
\begin{align*}
    M^\dagger {\left( M^{-1} \right)}^\dagger
    &= {\left( M^{-1} M \right)}^\dagger \\
    &= 1^\dagger \\
    &= 1,
\end{align*}
hence implying
\[
    {\left( M^{-1} \right)}^\dagger = {\left( M^\dagger \right)}^{-1}.
\]
\begin{align*}
    \therefore {\left( C^{-1} A C \right)}^\dagger
    &= C^{-1} A {\left( C^{-1} \right)}^\dagger \\
    &= C^{-1} A {\left( C^\dagger \right)}^{-1} \\
    &= C^{-1} A {C^{-1}}^{-1} \\
    &= C^{-1} A C
\end{align*}

\item
\begin{align*}
    {\left( C^{-1} D C \right)}^\dagger
    &= C^\dagger D^\dagger {\left( C^{-1} \right)}^\dagger \\
    &= C^{-1} D^{-1} {\left( C^\dagger \right)}^{-1} \\
    &= C^{-1} D^{-1} {\left( C^{-1} \right)}^{-1} \\
    &= {\left( C^{-1} D C \right)}^{-1}
\end{align*}

\item
\begin{align*}
    {\left( i (AB - BA) \right)}^\dagger
    &= i^* \left( B^\dagger A^\dagger - A^\dagger B^\dagger \right) \\
    &= -i (BA - AB) \\
    &= i (AB - BA)
\end{align*}

\end{enumerate}

