%%%%%%%%%%%%%%%%%%%%%%%
\item
%%%%%%%%%%%%%%%%%%%%%%%

\begin{enumerate}[wide, labelindent = 0pt, label = (\alph*)]
\item
The relation holds when $\mathbb{b} = \mathbb{0}$, as both sides are zero.
When $\mathbb{b} \neq \mathbb{0}$, define $\mathbb{c} := \mathbb{a} + \lambda \mathbb{b}$.
\begin{align*}
    0
    &\leq \mathbb{c} \cdot \mathbb{c} \\
    &= \left( \mathbb{a} + \lambda \mathbb{b} \right) \cdot \left( \mathbb{a} + \lambda \mathbb{b} \right) \\
    &= \mathbb{a} \cdot \mathbb{a}
     + 2\Re\left\{ \lambda \mathbb{a} \cdot \mathbb{b} \right\}
     + \mathbb{b} \cdot \mathbb{b} \lambda^2
\end{align*}
As this holds for any $\lambda$, let
\[
    \lambda = -\frac{\mathbb{b} \cdot \mathbb{a}}{\mathbb{b} \cdot \mathbb{b}}.
\]
\[
    \Rightarrow 0
    \leq \mathbb{a} \cdot \mathbb{a} - \frac{
        {\abs{\mathbb{a} \cdot \mathbb{b}}}^2
    }{\mathbb{b} \cdot \mathbb{b}}
\]
\[
    \therefore (\mathbb{a} \cdot \mathbb{a}) (\mathbb{b} \cdot \mathbb{b})
    \geq {\abs{\mathbb{a} \cdot \mathbb{b}}}^2
\]

\item
\[
    \mathbb{x} \cdot \mathbb{x}^{(n)}
    = \sum_{i = 1}^n x_i (\mathbb{x} \cdot \mathbb{e}_i)
    = \sum_{i = 1}^n {\abs{x_i}}^2
\]
\[
    \mathbb{x}^{(n)} \cdot \mathbb{x}^{(n)}
    = \sum_{i = 1}^n \sum_{j = 1}^n {\abs{x_i}}^2 \delta_{ij}
    = \sum_{i = 1}^n {\abs{x_i}}^2
\]
\[
    \Rightarrow \mathbb{x} \cdot \mathbb{x} \left(
        \sum_{i = 1}^n {\abs{x_i}}^2
    \right)
    = {\left(
       \sum_{i = 1}^n {\abs{x_i}}^2
    \right)}^2
\]
\[
    \therefore \mathbb{x} \cdot \mathbb{x} \geq \sum_{i = 1}^n {\abs{x_i}}^2
\]
(When $\sum_{i = 1}^n {\abs{x_i}}^2 = 0$, then the norm must be no less than 0.)
\end{enumerate}
