%%%%%%%%%%%%%%%%%%%%%%%
37.
%%%%%%%%%%%%%%%%%%%%%%%
We must evaluate the integral
\[
    \psi \left(\mathbb{k}, \mathbb{l} \right)
    := \int \frac{d\Omega}{\left( 1 + \mathbb{k} \cdot \unitvec{r} \right) \left( 1 + \mathbb{l} \cdot \unitvec{r} \right)}
\]
using Feynman's identity (\refeq{3}{28}).
\begin{align*}
    \Rightarrow \psi \left(\mathbb{k}, \mathbb{l} \right)
    &= \int d\Omega \int_0^1 du \inv{{\left(
        \left( 1 + \mathbb{k} \cdot \unitvec{r} \right) u
        + \left( 1 + \mathbb{l} \cdot \unitvec{r} \right) (1 - u)
    \right)}^2} \\
    &= \int_0^1 du \int \frac{d\Omega}{{\left(
        1 + \left(u \mathbb{k} + (1 - u) \mathbb{l}\right) \cdot \unitvec{r}
    \right)}^2}
\end{align*}

Let
\[
    F(\mathbb{v}) := \int \frac{d\Omega}{{\left( 1 + \mathbb{v} \cdot \unitvec{r} \right)}^2}.
\]
This scalar-valued integral is a function of a vector;
thus, it may only depend on the vector's magnitude.
Let $v := \norm{\mathbb{v}}$.
\begin{align*}
    \Rightarrow F(\mathbb{v})
    &= F \left( v \zhat \right) \\
    &= \int \frac{d\Omega}{{\left( 1 + vz \right)}^2} \\
    &= \int_0^\pi d\theta \int_0^{2\pi} d\phi \sin \theta \cdot \inv{{\left( 1 + v\cos \theta \right)}^2} \\
    &= 2\pi \diffBetween{\inv{v(1 + v \cos \theta)}}{0}{\pi} \\
    &= \frac{4\pi}{1 - v^2}
\end{align*}
\begin{align*}
    \Rightarrow \psi \left(\mathbb{k}, \mathbb{l} \right)
    &= \int_0^1 du F\left( u\mathbb{k} + (1 - u)\mathbb{l} \right) \\
    &= 4\pi \int_0^1 \frac{du}{1 - \norm{u\mathbb{k} + (1 - u)\mathbb{l}}^2} \\
    &= 4\pi \int_0^1 \frac{du}{
        1 - l^2
        - 2\left( \mathbb{k}\cdot\mathbb{l} - l^2 \right) u
        + \left( k^2 + l^2 - 2\mathbb{k}\cdot\mathbb{l} \right) u^2
    }
\end{align*}
where $k := \norm{\mathbb{k}}$ and $l := \norm{\mathbb{l}}$.
Now, notice that
\[
    \frac{d}{dx} \tanh^{-1} x = \inv{1 - x^2}.
\]
\begin{align*}
    \Rightarrow \inv{c - 2bx - ax^2}
    &=  \inv{\sqrt{ac + b^2}} \cdot \frac{\frac{a}{\sqrt{ac + b^2}}}{1 - {\left(
        \frac{a}{\sqrt{ac + b^2}} \left( x + \frac{b}{a} \right)
    \right)}^2} \\
    &= \frac{d}{dx} \left( \inv{\sqrt{ac + b^2}} \tanh^{-1} \left( \frac{ax + b}{\sqrt{ac + b^2}} \right) \right)
\end{align*}
\begin{align*}
    \Rightarrow \psi \left(\mathbb{k}, \mathbb{l} \right)
    &= \frac{4\pi}{\sqrt{
        {\left( 1 - \mathbb{k}\cdot\mathbb{l} \right)}^2
        - \left( 1 - k^2 \right) \left( 1 - l^2 \right)
    }} \\
    &\quad \times \diffBetween{\tanh^{-1} \left(
        \frac{
            \left( k^2 + l^2 - 2\mathbb{k}\cdot\mathbb{l} \right) u 
            + \mathbb{k}\cdot\mathbb{l} - l^2
        }{\sqrt{
             {\left( 1 - \mathbb{k}\cdot\mathbb{l} \right)}^2
            - \left( 1 - k^2 \right) \left( 1 - l^2 \right)
        }}
    \right)}{0}{1} \\
    &= \frac{4\pi}{\sqrt{A^2 - B^2}} \left(
        \tanh^{-1} \left( \frac{A - 1 + k^2}{\sqrt{A^2 - B^2}} \right)
        + \tanh^{-1} \left( \frac{A - 1 + l^2}{\sqrt{A^2 - B^2}} \right)
    \right)
\end{align*}
where $A := 1 - \mathbb{k}\cdot\mathbb{l}$ and $B := \sqrt{\left( 1 - k^2 \right) \left( 1 - l^2 \right)}$.

Now, note that
\begin{align*}
    \cosh \left( \tanh^{-1} x + \tanh^{-1} y \right)
    &= \cosh \left( \tanh^{-1} x \right) \cosh \left( \tanh^{-1} y \right) \\
    &\quad + \sin \left( \tanh^{-1} x \right) \sinh \left( \tanh^{-1} y \right) \\
    &= \inv{\left( 1 - x^2 \right)} \cdot \inv{\left( 1 - x^2 \right)}
     + \frac{x}{\left( 1 - x^2 \right)} \cdot \frac{y}{\left( 1 - y^2 \right)} \\
    &= \frac{1 + xy}{\sqrt{\left( 1 - x^2 \right) \left( 1 - y^2 \right)}}.
\end{align*}
In our case, we have
\[
    x = \frac{A - 1 + k^2}{\sqrt{A^2 - B^2}} \text{ and } y = \frac{A - 1 + l^2}{\sqrt{A^2 - B^2}}
\]
which yields
\[
    1 + xy = \frac{A}{A^2 - B^2} \left( 2A + k^2 + l^2 - 2 \right)
\]
and
\[
    \sqrt{\left( 1 - x^2 \right) \left( 1 - y^2 \right)}
    = \frac{B}{A^2 - B^2} \left( 2A + k^2 + l^2 - 2 \right).
\]
\[
    \Rightarrow \tanh^{-1} x + \tanh^{-1} y
    = \cosh^{-1} \left( \frac{1 + xy}{\sqrt{\left( 1 - x^2 \right) \left( 1 - y^2 \right)}} \right)
    = \cosh^{-1} \frac{A}{B}
\]
\[
    \therefore \psi \left(\mathbb{k}, \mathbb{l} \right)
    = \frac{4\pi}{\sqrt{A^2 - B^2}} \cosh^{-1} \frac{A}{B}
\]

