%%%%%%%%%%%%%%%%%%%%%%%
10.
%%%%%%%%%%%%%%%%%%%%%%%
\begin{enumerate}[wide, labelindent = 0pt, label = (\alph*)]
\item
\[
    \Re F(x)
    = \Re F(x_0)
    + \frac{x - x_0}{\pi} \Pint_{-\infty}^\infty dx' \frac{\Im F(x')}{(x' - x_0)(x' - x)}
\]
\[
    \Rightarrow \frac{\Re F(x) - \Re F(x_0)}{x - x_0}
    = \inv{\pi} \Pint_{-\infty}^\infty dx' \frac{\Im F(x')}{(x' - x_0)(x' - x)}
\]
\begin{align*}
    \xRightarrow{x_0 \rightarrow x} \Re F'(x)
    &= \inv{\pi} \Pint_{-\infty}^\infty dx' \frac{\Im F(x')}{{(x' - x)}^2} \\
    &= \inv{\pi} \left(
        \diffBetween{-\frac{\Im F(x')}{x' - x}}{-\infty}{\infty}
        + \int_{-\infty}^\infty dx' \frac{F'(x')}{x' - x}
    \right) \\
    &= \inv{\pi} \Pint_{-\infty}^\infty dx' \frac{F'(x')}{x' - x}
\end{align*}
Therefore, replacing $F'$ with $F$ and substituting $x = 0$ yields the desired sum rule.

\item
You substitute $x = 0$.
I really don't understand what the problem is here.

\item
\notyet\footnote{%
But my beef with this problem lies beyond the simple ``What should I do?'' confusion.
I feel like whatever we derived in part~(a) is a large nothing-burger;
it is simply the unsubtracted relation evaluated at $0$, as stated in part~(b).
What am I proving? What is the goal?
If we want to express some rule such as
\[
    \Re F(x) = \Pint dx' \Im F(x) \cdot (\text{something}),
\]
when what kind of properties are we trying to get for $(\text{something})$?
How close of an analogy are we talking about?
Could you tell I'm losing my mind here?
}

\end{enumerate}

